lib/DataStructures/LinearLru.i.dfy
@@ -1,0 +1,120 @@
+include "../Lang/NativeTypes.s.dfy"
+include "../Base/Option.s.dfy"
+include "../Base/DebugAccumulator.i.dfy"
+include "LruModel.i.dfy"
+include "LinearMutableMap.i.dfy"
+include "LinearDList.i.dfy"
+
+module LinearLru
+{
+  import opened NativeTypes
+  import opened Options
+  import LruModel`Internal
+  import LinearMutableMap
+  import DList
+  export
+    provides NativeTypes, Options, LruModel
+    provides LinearLru
+    provides Inv, Queue
+    provides Alloc, Free, Remove, Use, Next, NextOpt
+
+  linear datatype LinearLru = LinearLru(
+    linear dlist:DList.DList<uint64>,  // list of values
+    linear ptr_map:LinearMutableMap.LinearHashMap<uint64> // map of pointers into dlist
+    )
+
+  predicate Inv(lru:LinearLru) {
+    var q := DList.Seq(lru.dlist);
+    && LinearMutableMap.Inv(lru.ptr_map)
+    && DList.Inv(lru.dlist)
+    && LruModel.WF(q)
+    && LruModel.I(q) == lru.ptr_map.contents.Keys
+    && (forall i {:trigger q[i] in lru.ptr_map.contents} :: 0 <= i < |q| ==>
+      && q[i] in lru.ptr_map.contents
+      && DList.Index(lru.dlist, lru.ptr_map.contents[q[i]]) as int == i)
+    && (forall x :: x in lru.ptr_map.contents ==>
+      && DList.ValidPtr(lru.dlist, lru.ptr_map.contents[x])
+      && DList.Get(lru.dlist, lru.ptr_map.contents[x]) == x)
+  }
+
+  function Queue(lru:LinearLru):(q:LruModel.LruQueue)
+    ensures Inv(lru) ==> LruModel.WF(q)
+  {
+    DList.Seq(lru.dlist)
+  }
+
+  method Alloc() returns(linear lru:LinearLru)
+    ensures Inv(lru)
+  {
+    var size := 128;
+    linear var dlist := DList.Alloc<uint64>(size + 1);
+    linear var ptr_map := LinearMutableMap.Constructor(size);
+    lru := LinearLru(dlist, ptr_map);
+  }
+
+  method Free(linear lru:LinearLru)
+  {
+    linear var LinearLru(dlist, ptr_map) := lru;
+    DList.Free(dlist);
+    LinearMutableMap.Destructor(ptr_map);
+  }
+
+  method Remove(linear lru:LinearLru, x:uint64) returns(linear lru':LinearLru)
+    requires Inv(lru)
+    ensures Inv(lru')
+    ensures Queue(lru') == LruModel.Remove(Queue(lru), x)
+  {
+    linear var LinearLru(dlist, ptr_map) := lru;
+    ghost var q := DList.Seq(dlist);
+    LruModel.LruRemove'(q, x);
+
+    linear var RemoveResult(ptr_map', removed) := LinearMutableMap.RemoveAndGet(ptr_map, x);
+    if (removed.Some?) {
+      var Some(p) := removed;
+      dlist := DList.Remove(dlist, p);
+    }
+    lru' := LinearLru(dlist, ptr_map');
+  }
+
+  method Use(linear lru:LinearLru, x:uint64) returns(linear lru':LinearLru)
+    requires Inv(lru)
+    requires |LruModel.I(Queue(lru))| < 0x1_0000_0000_0000_0000 / 8
+    ensures Inv(lru')
+    ensures Queue(lru') == LruModel.Use(Queue(lru), x)
+  {
+    LruModel.QueueCount(Queue(lru));
+    LruModel.LruRemove'(Queue(lru), x);
+    lru' := Remove(lru, x);
+    LruModel.QueueCount(Queue(lru'));
+
+    linear var LinearLru(dlist, ptr_map) := lru';
+    var p;
+    dlist, p := DList.InsertBefore(dlist, 0, x);
+    ptr_map := LinearMutableMap.Insert(ptr_map, x, p);
+    lru' := LinearLru(dlist, ptr_map);
+  }
+
+  method Next(shared lru:LinearLru) returns(x:uint64)
+    requires Inv(lru)
+    requires |LruModel.I(Queue(lru))| > 0
+    ensures x == LruModel.Next(Queue(lru))
+  {
+    LruModel.QueueCount(DList.Seq(lru.dlist));
+    var p := DList.Next(lru.dlist, 0);
+    x := DList.Get(lru.dlist, p);
+  }
+
+  method NextOpt(shared lru:LinearLru) returns(x:Option<uint64>)
+    requires Inv(lru)
+    ensures x == LruModel.NextOpt(Queue(lru))
+  {
+    LruModel.QueueCount(DList.Seq(lru.dlist));
+    var p := DList.Next(lru.dlist, 0);
+    if (p == 0) {
+      x := None;
+    } else {
+      LruModel.reveal_NextOpt();
+      x := Some(DList.Get(lru.dlist, p));
+    }
+  }
+}
